WIP: seems stucked another construction

concur/VCompBig.v
@@ -126,6 +126,7 @@ Qed.
 
 
 (** ** Identity *)
+(*
 Program Instance world_unit : World unit :=
   {|
     w_state := unit;
@@ -147,7 +148,7 @@ Solve All Obligations with
   cbn; intros; subst; auto.
 
 Notation "1" := cc_id : gs_cc_scope.
-
+*)
 
 (** Algebraic structures on calling conventions. *)
 
@@ -159,21 +160,216 @@ Notation "1" := cc_id : gs_cc_scope.
   refined by the calling convention [cc'], meaning that any
   [cc']-simulation is also a [cc]-simulation. *)
 
-(*Section CCTRANS.
-
-  Context {li1 li2} (cc1 cc2: callconv li1 li2)
-    Context (se1)
-*)
 (** cc1: internal, i.e. injp ⋅ injp
     cc2: external, i.e. injp  *)
 
-(*
-Definition acci_future_query {li1 li2} {cc1 cc2: callconv li li2}
-  (wp1 : gworld cc1) (wp2 : gworld cc2) :=
-  forall wp1' w1 q1 q2, wp1 *-> wp1' /\ match_query cc1 w1 q1 q2 /\
+(* 
+Inductive same_mem {li1 li2: language_interface} {cc1 cc2: callconv li1 li2} : gworld cc1 -> gworld cc2 -> Prop :=
+|match_query_mem : forall w1 w2 q1 q2 wp1 wp2,
+    match_query cc1 w1 q1 q2 -> match_query cc2 w2 q1 q2 ->
+    get w1 = wp1 -> get w2 = wp2 ->
+    same_mem wp1 wp2
+|match_reply_mem : forall w1 w2 r1 r2 wp1 wp2,
+    match_reply cc1 w1 r1 r2 -> match_reply cc2 w2 r1 r2 ->
+    get w1 = wp1 -> get w2 = wp2 ->
+    same_mem wp1 wp2.
+
+Definition ACCI_12 {li1 li2} {cc1 cc2: callconv li1 li2} (wp1 : gworld cc1) (wp2 : gworld cc2) :=
+  forall wp1' wp2', wp1 *-> wp1' -> same_mem wp1' wp2' -> wp2 *-> wp2'.
  *)
 
+(** The passive outgoing : leaving wA2 as given*)
+Definition ccref_outgoing {li1 li2} (cc1 cc2: callconv li1 li2) :=
+  forall w1 se1 se2 q1 q2 w2,
+    match_senv cc1 w1 se1 se2 ->
+    match_query cc1 w1 q1 q2 ->
+    match_query cc2 w2 q1 q2 ->
+      forall r1 r2 (wp2: gworld cc2),
+        get w2 o-> wp2 ->
+        match_reply cc2 (set w2 wp2) r1 r2 ->
+        exists (wp1 : gworld cc1),
+        get w1 o-> wp1 /\
+         match_reply cc1 (set w1 wp1) r1 r2.
+(** I -> F *)
+Definition ccref_incoming {li1 li2} (cc1 cc2: callconv li1 li2) :=
+  forall w2 se1 se2 q1 q2,
+    match_senv cc2 w2 se1 se2 ->
+    match_query cc2 w2 q1 q2 ->
+    exists (w1: ccworld cc1) ,
+      match_senv cc1 w1 se1 se2 /\
+      match_query cc1 w1 q1 q2 /\
+      (* (forall (wp1': gworld cc1), get w1 *-> wp1' -> exists (wp2' : gworld cc2), get w2 *-> wp2'). *)
+      (* (forall q1 q2 (w1' : ccworld cc1) (wp1' : gworld cc1),  get w1' = wp1' -> (get w1) *-> wp1' ->  match_query cc1 w1' q1 q2 -> match_senv cc1 w1' se1 se2 ->
+                           exists (w2': ccworld cc2) (wp2' : gworld cc2), get w2' = wp2' /\ (get w2) *-> (get w2') /\ match_query cc2 w2' q1 q2 /\ match_senv cc2 w2' se1 se2) /\ *)
+      (forall r1 r2 (wp1: gworld cc1),
+        get w1 o-> wp1 -> (get w1 *-> wp1) ->
+        match_reply cc1 (set w1 wp1) r1 r2 ->
+        exists (wp2 : gworld cc2),
+        get w2 o-> wp2 /\ (get w2 o-> wp2) ->
+        match_reply cc2 (set w2 wp2) r1 r2).
 
+Record cctrans {li1 li2} (cc1 cc2: callconv li1 li2) :=
+    Callconv_Trans{
+        big_step_incoming : ccref_incoming cc1 cc2;
+        big_step_outgoing : ccref_outgoing cc1 cc2;
+      }.
+
+  
+  Lemma open_fsim_cctrans {li1 li2: language_interface}:
+  forall (cc1 cc2: callconv li1 li2) L1 L2,
+    forward_simulation cc1 L1 L2 ->
+    cctrans cc1 cc2 ->
+    forward_simulation cc2 L1 L2.
+  (*cc1 : injp @ injp cc2: injp*)
+Proof.
+  intros.
+  destruct H0 as [INCOM OUTGO].
+  inv H.
+  destruct X as [index order match_states SKEL PROP WF].
+  constructor.
+    set (ms se1 se2 (w2 : ccworld cc2) (wp2: gworld cc2) idx s1 s2 :=
+         exists w1 wp1,
+           match_states se1 se2 w1 wp1 idx s1 s2 /\
+             match_senv cc1 w1 se1 se2 /\
+             (forall q1 q2 (w1': ccworld cc1), wp1 *-> (get w1') -> match_query cc1 w1' q1 q2 -> match_senv cc1 w1' se1 se2 ->
+                           exists (w2' : ccworld cc2), wp2 *-> (get w2') /\ match_query cc2 w2' q1 q2 /\ match_senv cc2 w2' se1 se2) /\
+             (forall r1 r2 (wp1' : gworld cc1), (get w1) o-> wp1' -> wp1 *-> wp1' -> match_reply cc1 (set w1 wp1') r1 r2 ->
+                            exists (wp2' : gworld cc2), (get w2) o-> wp2' /\ wp2 *-> wp2' /\ match_reply cc2 (set w2 wp2') r1 r2)).
+  eapply Forward_simulation with order ms; auto.
+  intros se1 se2 wB' Hse' Hse1.
+  split.
+  - intros q1 q2 Hq'.
+    destruct (INCOM wB' se1 se2 q1 q2) as (wB & Hse & Hq & Hr); auto.
+    eapply fsim_match_valid_query; eauto.
+  - intros q1 q2 s1 Hq' Hs1 Ho.
+    destruct (INCOM wB' se1 se2 q1 q2) as (wB & Hse & Hq & Hxy & Hf); auto.
+    edestruct @fsim_match_initial_states as (i & s2 & Hs2 & Hs); eauto.
+    exists i, s2. split; auto. red. exists wB,(get wB). repeat apply conj; eauto.
+    + intros. (* Set Printing All. *)
+      simpl in *. eapply Hxy in H0. eapply H0 in exploit Hxy; eauto. 
+    intuition auto. 
+    admit. admit.
+  - intros gw i s1 s2 r1 (wB & gw' & Hs & Hse & Hxy & Hf) Hr1.
+    edestruct @fsim_match_final_states as (r2 & gw1 & Hr2 & ACCO1 & ACCI1 & Hr); eauto.
+    exploit Hf; eauto. intros (gw2 &  ACCO2 & Hr2'). exists r2.
+    exists gw2. intuition auto.
+  - (*the most tricky part*)
+    intros gw2 i s1 s2 qA1 (wB & gw1 & Hs & Hse & Hxy & Hf) HqA1.
+    edestruct @fsim_match_external as (wA & qA2 & Hacc1 & HqA2 & HqA & HseA & ?); eauto.
+    edestruct Hxy as (wA' & Hacci & Hq & Hsea); eauto.
+    specialize (OUTGO _ _ _ _ _ _ HseA HqA Hq) as Hroutgo.
+    exists wA', qA2. intuition auto.
+    exploit Hroutgo; eauto. intros (wp1 & ACCO1 & MR1).
+    edestruct H as (i' & s2' & Hs2' & Hs'); eauto.
+    exists i', s2'. split; auto.
+    exists wB, wp1. repeat apply conj; eauto.
+    admit. admit.
+  - intros s1 t s1' Hs1' gw2 i s2 (wB & gw1 & Hs & Hse & Hr').
+   edestruct @fsim_simulation as (i' & s2' & Hs2' & Hs'); eauto.
+    exists i', s2'. split; auto.
+    econstructor; eauto.
+Qed.
+
+
+(** TODOs*)
+(** 1.Definition of c_injp as a callconv *)
+(** 2.Achieve [cctrans (injp@injp) (injp)] *)
+(** 3.Introduce callconv with empty world (ext, inj, CLLMMA) *)
+(** 4.Try the composition of these trivial callconv using cctrans *)
+(** 4.1 The self-simulation mechniasm? *)  
+(** 4.Modify the proofs of each pass *)
+(** 5.Compose the compiler *)
+
+  
+Require Import Inject InjectFootprint.
+
+Program Instance injp_world_id : World injp_world :=
+    {
+      w_state := injp_world;
+      w_lens := lens_id;
+      w_acci := injp_acci;
+      w_acce := injp_acce;
+      w_acci_trans := injp_acci_preo;
+    }.
+
+Program Definition c_injp : callconv li_c li_c :=
+  {|
+    ccworld := injp_world;
+    ccworld_world := injp_world_id;
+    match_senv w := CKLR.match_stbls injp w;
+    match_query := cc_c_query injp;
+    match_reply := cc_c_reply injp;    
+  |}.
+Next Obligation.
+  inv H. inv H0. auto.
+Qed.
+Next Obligation.
+  intros. inv H. erewrite <- Genv.valid_for_match; eauto.
+Qed.
+
+Compute (ccworld (cc_compose c_injp c_injp)).
+
+Lemma cctrans_injp_comp : cctrans (cc_compose c_injp c_injp) (c_injp).
+Proof.
+  econstructor.
+  - (*incoming construction*)
+    red. intros. inv H0. inv H3. simpl in H2, H1.
+    inv H.
+    exists (se1, (injpw (meminj_dom f) m1 m1 (mem_inject_dom f m1 m2 Hm),
+              injpw f m1 m2 Hm)).
+    repeat apply conj; eauto.
+    + simpl. split. constructor; eauto. eapply match_stbls_dom; eauto. constructor; simpl; eauto.
+    + exists (cq vf1 sg vargs1 m1). split.
+      econstructor; simpl; eauto. eapply val_inject_dom; eauto.
+      eapply val_inject_list_dom; eauto.
+      econstructor; eauto. simpl. econstructor; eauto.
+    + red. simpl. intros.
+      red in H. inv H0.
+      -- destruct w1 as [se1' [w11 w12]]. simpl. simpl in H.
+         inv H3. inv H5. destruct H as [ACCI1 ACCI2].
+         destruct H0 as [Hq1 Hq2]. inv Hq1. inv Hq2.
+         simpl in *. inv H8. inv H16. inv H22.
+         rename m0 into m1'. rename m3 into m2'. rename m5 into m3'.
+         rename f0 into f'.
+         inv ACCI1. inv ACCI2.
+         assert (Hcom: f' = compose_meminj f1 f2). admit.
+         constructor; eauto.
+         ++ inv H24. split. eauto.
+            eapply Mem.unchanged_on_implies. eauto.
+            intros. destruct H. split. red. red in H.
+            unfold meminj_dom. rewrite H. auto. auto.
+         ++ red. intros. simpl in *.
+            clear - Hm6 Hm9 Hm12 H26 H34 H Hm0 Hcom.
+            rewrite Hcom. unfold compose_meminj.
+            assert (Hf0 : (meminj_dom f) b = Some (b,0) ).
+            unfold meminj_dom. rewrite H. reflexivity.
+            apply H26 in Hf0. rewrite Hf0.
+            apply H34 in H. rewrite H. reflexivity.
+         ++ admit. (* ok *)
+      -- admit. (*same as the match_query part *)
+    + intros r1 r3 wp1 [Hae1 Hae2] Hr. simpl in Hae1, Hae2.
+      simpl in wp1. destruct wp1 as [wp11 wp12].
+      simpl in *. destruct Hr as [r2 [Hr1 Hr2]].
+      admit. (*just compose wp11 and wp12*)
+  - (* outgoing construction *)
+    red. intros.
+        ;
+Admitted.
+
+Theorem injp_pass_compose: forall (L1 L2 L3: semantics li_c li_c),
+    forward_simulation c_injp L1 L2 ->
+    forward_simulation c_injp L2 L3 ->
+    forward_simulation c_injp L1 L3.
+Proof.
+  intros.
+  assert (forward_simulation (cc_compose c_injp c_injp) L1 L3).
+  eapply st_fsim_vcomp; eauto.
+  eapply open_fsim_cctrans; eauto.
+  apply cctrans_injp_comp.
+Qed.
+
+
+(** *
 Inductive same_mem {li1 li2: language_interface} {cc1 cc2: callconv li1 li2} : gworld cc1 -> gworld cc2 -> Prop :=
 |match_query_mem : forall w1 w2 q1 q2 wp1 wp2,
     match_query cc1 w1 q1 q2 -> match_query cc2 w2 q1 q2 ->
@@ -375,5 +571,5 @@ Proof.
   apply cctrans_injp_comp.
 Qed.
 
-
+*)
 
